\pd{\rho}{t} + \nabla \cdot (\rho\vec{v}) = 0
\frac{\Dif\vec{v}}{\Dif t} = -\frac{\nabla p}{\rho} + \nu\nabla^2\vec{v} + \vec{F}
\frac{\Dif\theta}{\Dif t} = \frac{1}{c_p} + \del{\frac{\theta}{T}}\dot{Q}
\pd{p}{z} = -\rho g
p = \rho R T
\dif I = T\dif \eta -p\dif\alpha + \mu\dif S
c_p = c_v + R
\dif Q = c_p \dif T - \alpha\dif p
\theta = T\intoo{\frac{p_0}{p}}^\kappa
B = \frac{\vec{v}^2}{2} + c_p T + gz = const
\vec{F}_{Co} = -2\vec{\Omega}\times\vec{v}_R
f = 2\omega sin\phi
N^2 = -\frac{g}{\tilde{\rho}}\pd{\tilde{\rho}}{z}
\Gamma_d = \frac{g}{c_p}
\od{e_s}{T} = \frac{L_c e_s}{R_v T^2}
\omega^2 = \frac{K^2 N^2}{k^2 + m^2}
Ek = \del{\frac{A}{f_0 H^2}}
Ro \equiv \frac{U}{fL}
\vec{f}\times{u} \approx -\frac{1}{\rho}\nabla_z p
N^2 = -\frac{g}{\tilde{\rho}}\pd{\tilde{\rho}}{z}
APE = \frac{R\overline{p}_{S}^{-\kappa}}{2}\int^{p_S}_{0}p^{\kappa-1}\intoo{-g\pd{\overline{\theta}}{p}}\overline{\theta^{\prime 2}} \dif p
\vec{\omega} = \nabla\times \vec{v}
C = \oint\vec{v}\cdot \dif\vec{l}
\frac{\Dif}{\Dif t}\oint\vec{v}\cdot \dif\vec{r}
\frac{\Dif}{\Dif t}(\zeta + f) = -(\zeta + f)\intoo{\pd{u}{x} + \pd{v}{y}} + \intoo{\pd{u}{z}\pd{w}{y} - \pd{v}{z}\pd{w}{x}} + \frac{1}{\rho^2}\intoo{\pd{\rho}{x}\pd{p}{y}-\pd{\rho}{y}\pd{p}{x}} + \intoo{\pd{F_y}{x}-\pd{F_x}{y}}
\frac{\Dif}{\Dif t}\intoo{\frac{\vec{\omega}_a \cdot \nabla\theta}{\rho}} = 0
Bu = \intoo{\frac{Ro}{Fr}}^2
\intoo{U-c}\intoo{\tilde{\psi}_{yy} - k^2\tilde{\psi}} + \intoo{\beta - U_{yy}}\tilde{\psi} = 0
\sigma \sim \frac{U}{L_d} = \Lambda\frac{f_0}{N}
q = \beta y + \intcc{\nabla^2 + \pd{}{z}\intoo{\frac{f_0^2}{N^2}\pd{}{z}}}\psi
\mathcal{F} = -\overline{u'v'}\vec{j} + \frac{f_0}{N^2}\overline{v'b'}\vec{k}
\pd{\mathcal{A}}{t} + \nabla\cdot\vec{\mathcal{F}} = \mathcal{D}
\psi' = Re\Psi e^{i(kx+ly+mz-\omega t)}
\omega = \overline{u}k - \frac{\beta k}{\kappa^2}
\pd{}{t}\cbr{ \iint\frac{1}{2}\frac{\overline{q'^2}}{\partial_y\overline{q}}\dif y\dif z - \int\intcc{\frac{1}{2}\frac{f_0}{N^2}\frac{\overline{b'^2}}{\partial_y\overline{b}}}^H_0\dif y} = 0
\mathcal{E}(k) = \mathcal{K}\epsilon^{2/3}k^{-5/3}
L_v \sim \del{ \frac{\nu^3}{\epsilon} }^{1/4}
m = (u + \Omega r cos\vartheta)rcos\vartheta
\theta = \theta(0) - \frac{\theta_0\Omega^2y^4}{2gHa^2}
f_0(\vec{u}_1 - \vec{u}_2) = g'\vec{k}\times\nabla\eta
